books/tools/arith4-theory.lisp
@@ -1,0 +1,35 @@
+
+
+
+(in-package "ACL2")
+
+(defun before-arithmetic () nil)
+
+(table pre-arith4-theory-invariants nil
+       (table-alist 'theory-invariant-table world)
+       :clear)
+
+(include-book "arithmetic-4/top" :dir :system)
+(include-book "tools/rulesets" :dir :system)
+
+(def-ruleset! arith4-enable-ruleset (set-difference-theories
+                                     (current-theory :here)
+                                     (current-theory
+                                      'before-arithmetic)))
+
+(def-ruleset! arith4-disable-ruleset (set-difference-theories
+                                      (current-theory 'before-arithmetic)
+                                      (current-theory :here)))
+
+
+(table post-arith4-theory-invariants nil
+       (table-alist 'theory-invariant-table world)
+       :clear)
+
+(table theory-invariant-table nil
+       (table-alist 'pre-arith4-theory-invariants world)
+       :clear)
+
+(in-theory (e/d* () ((:ruleset arith4-enable-ruleset))
+                 ((:ruleset arith4-disable-ruleset))))
+
