books/tools/rulesets.lisp
@@ -1,0 +1,178 @@
+
+
+(in-package "ACL2")
+
+(program)
+
+
+(defun get-ruleset (name world)
+  (let* ((ruleset-alist (table-alist 'ruleset-table world)))
+    (cdr (assoc name ruleset-alist))))
+
+(defmacro ruleset (name)
+  `(get-ruleset ,name world))
+
+(defun is-ruleset (name world)
+  (let* ((ruleset-alist (table-alist 'ruleset-table world)))
+    (consp (assoc name ruleset-alist))))
+
+(defun ruleset-designatorp (x world)
+  (cond ((or (symbolp x)
+             (and (consp x)
+                  (not (keywordp (car x)))))
+         (theoryp! (list x) world))
+        ((runep x world) t)
+        ((and (consp x)
+              (consp (cdr x))
+              (not (cddr x))
+              (eq (car x) :ruleset))
+         (or (is-ruleset (cadr x) world)
+             (cw "**NOTE**:~%~x0 is not a ruleset.~%" (cadr x))))
+        (t (cw "**NOTE**:~%~x0 is not a valid ruleset designator.~%" x))))
+
+(defun ruleset-designator-listp (x world)
+  (if (atom x)
+      (eq x nil)
+    (and (ruleset-designatorp (car x) world)
+         (ruleset-designator-listp (cdr x) world))))
+
+
+
+
+
+(defmacro def-ruleset (name form)
+  (declare (xargs :guard (symbolp name)))
+  `(make-event
+    (let ((world (w state))
+          (name ',name))
+      (if (is-ruleset name world)
+          (er soft 'def-ruleset
+              "~x0 is already a ruleset.  Use add-to-ruleset or def-ruleset! ~
+               instead.~%" name)
+        (let ((result ,form))
+          (if (ruleset-designator-listp result world)
+              (value `(table ruleset-table ',name ',result))
+            (er soft 'def-ruleset "Invalid ruleset specified~%")))))))
+
+(defmacro add-to-ruleset (name form)
+  (declare (xargs :guard (symbolp name)))
+  `(make-event
+    (let ((world (w state))
+          (name ',name))
+      (if (is-ruleset name world)
+          (let ((result ,form))
+            (if (ruleset-designator-listp result world)
+                (value `(table ruleset-table ',name
+                               (union-equal ',result (ruleset ',name))))
+              (er soft 'add-to-ruleset "Invalid ruleset specified~%")))
+        (er soft 'add-to-ruleset
+            "~x0 is not already a ruleset.  Use def-ruleset, def-ruleset! ~
+             or add-to-ruleset! instead.~%" name)))))
+
+(defmacro def-ruleset! (name form)
+  (declare (xargs :guard (symbolp name)))
+  `(make-event
+    (let* ((world (w state))
+           (result ,form))
+      (if (ruleset-designator-listp result world)
+          (value `(table ruleset-table ',',name ',result))
+        (er soft 'def-ruleset! "Invalid ruleset specified~%")))))
+
+(defmacro add-to-ruleset! (name form)
+  (declare (xargs :guard (symbolp name)))
+  `(make-event
+    (let* ((world (w state))
+           (result ,form))
+      (if (ruleset-designator-listp result world)
+          (value `(table ruleset-table ',',name
+                         (union-equal ',result (ruleset ',name))))
+        (er soft 'add-to-ruleset! "Invalid ruleset specified~%")))))
+
+
+;; This is fragile; we don't recursively check rulesets that we're expanding.
+(defun expand-ruleset1 (x world)
+  (if (atom x)
+      nil
+    (let ((des (car x)))
+      (if (and (consp des)
+               (eq (car des) :ruleset))
+          (append (expand-ruleset1 (ruleset (cadr des)) world)
+                  (expand-ruleset1 (cdr x) world))
+        (cons (car x)
+              (expand-ruleset1 (cdr x) world))))))
+
+(defun expand-ruleset (x world)
+  (if (ruleset-designator-listp x world)
+      (expand-ruleset1 x world)
+    (er hard 'expand-ruleset "~x0 is not a valid ruleset.~%" x)))
+
+
+(defmacro enable* (&rest x)
+  `(union-theories-fn
+    (current-theory :here)
+    (expand-ruleset ',x world)
+    t world))
+
+(defmacro disable* (&rest x)
+  `(set-difference-theories-fn
+    (current-theory :here)
+    (expand-ruleset ',x world)
+    t world))
+
+
+(defun e/d*-fn (theory e/d-list enable-p)
+  (declare (xargs :guard (and (true-list-listp e/d-list)
+                              (or (eq enable-p t)
+                                  (eq enable-p nil)))))
+  (cond ((atom e/d-list) theory)
+        (enable-p (e/d*-fn `(UNION-THEORIES ,theory
+                                           (expand-ruleset ',(car e/d-list) world))
+                           (cdr e/d-list) nil))
+        (t (e/d*-fn `(SET-DIFFERENCE-THEORIES ,theory
+                                              (expand-ruleset ',(car e/d-list) world))
+                    (cdr e/d-list) t))))
+
+(defmacro e/d* (&rest theories)
+  (declare (xargs :guard (true-list-listp theories)))
+  (cond ((atom theories) '(current-theory :here))
+        (t (e/d*-fn '(current-theory :here)
+                    theories t))))
+
+(defmacro ruleset-theory (ruleset)
+  `(expand-ruleset (ruleset ,ruleset) world))
+
+
+#||
+;; I'm commenting this out because I don't want the tools directory to depend
+;; on the make-event directory.  - Sol
+
+(logic)
+
+(local
+ (encapsulate
+  nil
+  (include-book "make-event/assert" :dir :system)
+
+ (def-ruleset! foo '(append reverse))
+
+ (def-ruleset! bar '((:ruleset foo) nth))
+
+ (add-to-ruleset foo '((consp)))
+
+ (in-theory (enable* (:ruleset foo)))
+
+ (assert! (let ((ens (ens state)))
+            (active-runep '(:definition binary-append))))
+
+ (in-theory (disable* (:ruleset bar)))
+
+ (assert! (let ((ens (ens state)))
+            (not (active-runep '(:definition binary-append)))))
+
+ (in-theory (e/d* ((:ruleset bar)) ((:ruleset foo))))
+
+ (assert! (let ((ens (ens state)))
+            (and (not (active-runep '(:definition binary-append)))
+                 (active-runep '(:definition nth)))))))
+
+||#
