books/tools/stobj-help.lisp
@@ -1,0 +1,509 @@
+
+(in-package "ACL2")
+
+
+(defthm nth-out-of-range
+  (implies (<= (len lst) (nfix n))
+           (not (nth n lst))))
+
+(defthm len-resize-list
+  (equal (len (resize-list lst n default))
+         (nfix n)))
+
+(defun nth-rsz-induction (n len lst)
+  (if (or (zp n) (zp len))
+      lst
+    (nth-rsz-induction (1- n) (1- len)
+                       (if (consp lst) (cdr lst) lst))))
+
+
+(defthm nth-resize-list-nil
+  (implies (<= (nfix len) (nfix n))
+           (equal (nth n (resize-list lst len default)) nil))
+  :hints (("goal" :induct (nth-rsz-induction n len lst))))
+
+(defthm nth-resize-list
+  (equal (nth n (resize-list lst len default))
+         (and (< (nfix n) (nfix len))
+              (if (< (nfix n) (len lst))
+                  (nth n lst)
+                default)))
+  :hints (("goal" :induct (nth-rsz-induction n len lst)
+           :in-theory (enable zp len))
+          ("Subgoal *1/1"
+           :expand ((resize-list lst len default)
+                    (len lst)))))
+
+(defun nth-make-list-ac-ind (m n)
+  (if (or (zp m) (zp n))
+      nil
+    (nth-make-list-ac-ind (1- m) (1- n))))
+
+(defthmd make-list-ac-open
+  (implies (not (zp n))
+           (equal (make-list-ac n elt tail)
+                  (cons elt (make-list-ac (1- n) elt tail)))))
+
+(encapsulate
+ nil
+ (local (include-book "arithmetic-4/top" :dir :system))            
+ (defthm nth-make-list-ac
+   (equal (nth m (make-list-ac n elt tail))
+          (if (< (nfix m) (nfix n))
+              elt
+            (nth (- (nfix m) (nfix n)) tail)))
+   :hints (("goal" :induct (nth-make-list-ac-ind m n)
+            :in-theory (enable make-list-ac-open)))))
+
+(include-book "misc/simplify-thm" :dir :system)
+
+(program) (set-state-ok t)
+
+(defun array-specp (spec)
+  (let ((type (cadr (assoc-keyword :type (cdr spec)))))
+    (and (consp type)
+         (eq (car type) 'array))))
+
+(defun ht-specp (spec)
+  (let ((type (cadr (assoc-keyword :type (cdr spec)))))
+    (and (consp type)
+         (eq (car type) 'hash-table))))
+
+
+
+(defun mutator-calls (spec stobj renaming)
+  (let ((field (car spec)))
+    (cond
+     ((ht-specp spec)
+      `((,(defstobj-fnname field :updater :hash-table renaming) mk v ,stobj)
+        (,(defstobj-fnname field :remove :hash-table renaming) mk ,stobj)
+        (,(defstobj-fnname field :clear :hash-table renaming) ,stobj)))
+     ((array-specp spec)
+      `((,(defstobj-fnname field :updater :array renaming) mi v ,stobj)
+        (,(defstobj-fnname field :resize :array renaming) len ,stobj)))
+     (t
+      `((,(defstobj-fnname field :updater nil renaming) v ,stobj))))))
+
+(defun accessor-calls (spec stobj renaming)
+  (let ((field (car spec)))
+    (cond
+     ((ht-specp spec)
+      `((,(defstobj-fnname field :accessor :hash-table renaming) ak ,stobj)
+        (,(defstobj-fnname field :boundp :hash-table renaming) ak ,stobj)
+;; Leave out the get? function because we prefer to just expand its definition.
+;;        (,(defstobj-fnname field :accessor? :hash-table renaming) ak ,stobj)
+        (,(defstobj-fnname field :count :hash-table renaming) ,stobj)))
+     ((array-specp spec)
+      `((,(defstobj-fnname field :accessor :array renaming) ai ,stobj)
+        (,(defstobj-fnname field :length :array renaming) ,stobj)))
+     (t
+      `((,(defstobj-fnname field :accessor nil renaming) ,stobj))))))
+
+(defun def-stobj-self-mod-thms (spec stobj renaming)
+  (let ((field (car spec))
+        (create (defstobj-fnname stobj :creator nil renaming))
+        (init (cadr (assoc-keyword :initially (cdr spec)))))
+    (cond
+     ((ht-specp spec)
+      (let* ((upd (defstobj-fnname field :updater :hash-table renaming))
+             (rem (defstobj-fnname field :remove :hash-table renaming))
+             (clr (defstobj-fnname field :clear :hash-table renaming))
+             (acc (defstobj-fnname field :accessor :hash-table renaming))
+             (bdp (defstobj-fnname field :boundp :hash-table renaming))
+             (cnt (defstobj-fnname field :count :hash-table renaming)))
+        ;; Hoo boy.
+        `((defthm ,(incat stobj (symbol-name stobj) "-"
+                          (symbol-name acc) "-"
+                          (symbol-name create))
+            (equal (,acc ak (,create)) nil))
+          (defthm ,(incat stobj (symbol-name stobj) "-"
+                          (symbol-name acc) "-"
+                          (symbol-name upd))
+            (equal (,acc ak (,upd mk v ,stobj))
+                   (if (equal ak mk)
+                       v
+                     (,acc ak ,stobj))))
+          (defthm ,(incat stobj  (symbol-name stobj) "-"
+                          (symbol-name acc) "-"
+                          (symbol-name rem))
+            (equal (,acc ak (,rem mk ,stobj))
+                   (if (equal ak mk)
+                       nil
+                     (,acc ak ,stobj))))
+          (defthm ,(incat stobj  (symbol-name stobj) "-"
+                          (symbol-name acc) "-"
+                          (symbol-name clr))
+            (equal (,acc ak (,clr ,stobj))
+                   nil))
+          (defthm ,(incat stobj (symbol-name stobj) "-"
+                          (symbol-name bdp) "-"
+                          (symbol-name create))
+            (equal (,bdp ak (,create)) nil))
+          (defthm ,(incat stobj  (symbol-name stobj) "-"
+                          (symbol-name bdp) "-"
+                          (symbol-name upd))
+            (equal (,bdp ak (,upd mk v ,stobj))
+                   (if (equal ak mk)
+                       t
+                     (,bdp ak ,stobj))))
+          (defthm ,(incat stobj  (symbol-name stobj) "-"
+                          (symbol-name bdp) "-"
+                          (symbol-name rem))
+            (equal (,bdp ak (,rem mk ,stobj))
+                   (if (equal ak mk)
+                       nil
+                     (,bdp ak ,stobj))))
+          (defthm ,(incat stobj  (symbol-name stobj) "-"
+                          (symbol-name bdp) "-"
+                          (symbol-name clr))
+            (equal (,bdp ak (,clr ,stobj))
+                   nil))
+          (defthm ,(incat stobj (symbol-name stobj) "-"
+                          (symbol-name cnt) "-"
+                          (symbol-name create))
+            (equal (,cnt (,create)) 0))
+          (defthm ,(incat stobj  (symbol-name stobj) "-"
+                          (symbol-name cnt) "-"
+                          (symbol-name upd))
+            (equal (,cnt (,upd mk v ,stobj))
+                   (if (,bdp mk ,stobj)
+                       (,cnt ,stobj)
+                     (+ 1 (,cnt ,stobj)))))
+          (defthm ,(incat stobj  (symbol-name stobj) "-"
+                          (symbol-name cnt) "-"
+                          (symbol-name rem))
+            (equal (,cnt (,rem mk ,stobj))
+                   (if (,bdp mk ,stobj)
+                       (- (,cnt ,stobj) 1)
+                     (,cnt ,stobj))))
+          (defthm ,(incat stobj  (symbol-name stobj) "-"
+                          (symbol-name cnt) "-"
+                          (symbol-name clr))
+            (equal (,cnt (,clr ,stobj)) 0)))))
+     ((array-specp spec)
+      (let* ((upd (defstobj-fnname field :updater :array renaming))
+             (rsz (defstobj-fnname field :resize :array renaming))
+             (acc (defstobj-fnname field :accessor :array renaming))
+             (len (defstobj-fnname field :length :array renaming))
+             (size (car (caddr (cadr (assoc-keyword :type (cdr spec)))))))
+        `((defthm ,(incat stobj (symbol-name stobj) "-"
+                          (symbol-name acc) "-"
+                          (symbol-name create))
+            (equal (,acc ai (,create))
+                   (and (< (nfix ai) ,size) ,init))
+            :hints (("Goal" :in-theory (disable make-list-ac
+                                                (make-list-ac)))))
+          (defthm ,(incat stobj (symbol-name stobj) "-"
+                          (symbol-name acc) "-OUT-OF-RANGE")
+            (implies (<= (,len ,stobj) (nfix n))
+                     (not (,acc n ,stobj))))
+          (defthm ,(incat stobj (symbol-name stobj) "-"
+                          (symbol-name acc) "-NON-NATP")
+            (implies (not (natp n))
+                     (equal (,acc n ,stobj)
+                            (,acc 0 ,stobj))))
+          (defthm ,(incat stobj (symbol-name stobj) "-"
+                          (symbol-name acc) "-"
+                          (symbol-name upd))
+            (equal (,acc ai (,upd mi v ,stobj))
+                   (if (equal (nfix ai) (nfix mi))
+                       v
+                     (,acc ai ,stobj))))
+          (defthm ,(incat stobj (symbol-name stobj) "-"
+                          (symbol-name upd) "-NON-NATP")
+            (implies (not (natp n))
+                     (equal (,upd n v ,stobj)
+                            (,upd 0 v ,stobj))))
+          (defthm ,(incat stobj (symbol-name stobj) "-"
+                          (symbol-name acc)
+                          (symbol-name rsz))
+            (equal (,acc ai (,rsz len ,stobj))
+                   (and (< (nfix ai) (nfix len))
+                        (if (< (nfix ai) (,len ,stobj))
+                            (,acc ai ,stobj)
+                          ,init))))
+          (defthm ,(incat stobj (symbol-name stobj) "-"
+                          (symbol-name len) "-"
+                          (symbol-name create))
+            (equal (,len (,create)) ,size))
+          (defthm ,(incat stobj (symbol-name stobj) "-"
+                          (symbol-name len) "-"
+                          (symbol-name upd))
+            (equal (,len (,upd mi v ,stobj))
+                   (max (+ 1 (nfix mi)) (,len ,stobj))))
+          (defthm ,(incat stobj (symbol-name stobj) "-"
+                          (symbol-name len) "-"
+                          (symbol-name rsz))
+            (equal (,len (,rsz len ,stobj))
+                   (nfix len))))))
+     (t (let* ((upd (defstobj-fnname field :updater nil renaming))
+               (acc (defstobj-fnname field :accessor nil renaming)))
+          `((defthm ,(incat stobj (symbol-name stobj) "-"
+                            (symbol-name acc) "-"
+                            (symbol-name create))
+              (equal (,acc (,create)) ,init))
+            (defthm ,(incat stobj (symbol-name stobj) "-"
+                            (symbol-name acc) "-"
+                            (symbol-name upd))
+              (equal (,acc (,upd v ,stobj)) v))))))))
+
+(defun def-stobj-acc-of-upd-thms1111 (stobj acc upds)
+  (if (atom upds)
+      nil
+    (cons `(defthm ,(incat stobj (symbol-name stobj) "-"
+                           (symbol-name (car acc)) "-"
+                           (symbol-name (caar upds)))
+             (equal ,(subst (car upds) stobj acc)
+                    ,acc))
+          (def-stobj-acc-of-upd-thms1111 stobj acc (cdr upds)))))
+
+(defun def-stobj-acc-of-upd-thms111 (stobj accs upds)
+  (if (atom accs)
+      nil
+    (append (def-stobj-acc-of-upd-thms1111 stobj (car accs) upds)
+            (def-stobj-acc-of-upd-thms111 stobj (cdr accs) upds))))
+
+(defun def-stobj-acc-of-upd-thms11 (stobj spec specs renaming)
+  (if (atom specs)
+      nil
+    (append (if (equal spec (car specs))
+                (def-stobj-self-mod-thms spec stobj renaming)
+              (def-stobj-acc-of-upd-thms111
+                stobj
+                (accessor-calls spec stobj renaming)
+                (mutator-calls (car specs) stobj renaming)))
+            (def-stobj-acc-of-upd-thms11 stobj spec (cdr specs) renaming))))
+
+(defun def-stobj-acc-of-upd-thms1 (stobj specs all-specs renaming)
+  (if (atom specs)
+      nil
+    (append (def-stobj-acc-of-upd-thms11 stobj (car specs) all-specs renaming)
+            (def-stobj-acc-of-upd-thms1 stobj (cdr specs) all-specs
+              renaming))))
+
+(defun def-stobj-acc-of-upd-thms-mkevent (stobj state)
+  (let* ((rb (getprop stobj 'redundancy-bundle nil 'current-acl2-world
+                      (w state)))
+         (specs (car rb))
+         (renaming (cdr rb)))
+    (def-stobj-acc-of-upd-thms1 stobj specs specs renaming)))
+
+(defmacro def-stobj-acc-of-upd-thms (stobj)
+  `(make-event
+    `(progn . ,(def-stobj-acc-of-upd-thms-mkevent ',stobj state))))
+
+
+
+
+
+
+
+(defun def-stobj-type-theory-fn (stobj specs renaming state)
+  (declare (xargs :mode :program))
+  (if (atom specs)
+      (value nil)
+    (er-let*
+     ((thms
+       (let* ((spec (car specs))
+              (field (car spec)))
+         (cond
+          ((ht-specp spec)
+           (let* ((upd (defstobj-fnname field :updater :hash-table renaming))
+                  (rem (defstobj-fnname field :remove :hash-table renaming))
+                  (clr (defstobj-fnname field :clear :hash-table renaming))
+                  (bdp (defstobj-fnname field :boundp :hash-table renaming))
+                  (cnt (defstobj-fnname field :count :hash-table renaming))
+                  (stobj-rec
+                   (defstobj-fnname stobj :recognizer :top renaming)))
+             (value
+              `((defthm ,(incat stobj (symbol-name stobj) "-BOOLEANP-"
+                                (symbol-name bdp))
+                  (booleanp (,bdp ak ,stobj))
+                  :rule-classes :type-prescription)
+                (defthm ,(incat stobj (symbol-name stobj) "-NATP-"
+                                (symbol-name cnt))
+                  (natp (,cnt ,stobj))
+                  :rule-classes :type-prescription)
+                (defthm ,(incat stobj (symbol-name stobj-rec) "-"
+                                (symbol-name upd))
+                  (implies (,stobj-rec ,stobj)
+                           (,stobj-rec (,upd mk v ,stobj))))
+                (defthm ,(incat stobj (symbol-name stobj-rec) "-"
+                                (symbol-name rem))
+                  (implies (,stobj-rec ,stobj)
+                           (,stobj-rec (,rem mk ,stobj))))
+                (defthm ,(incat stobj (symbol-name stobj-rec) "-"
+                                (symbol-name clr))
+                  (implies (,stobj-rec ,stobj)
+                           (,stobj-rec (,clr ,stobj))))))))
+          ((array-specp spec)
+           (let* ((upd (defstobj-fnname field :updater :array renaming))
+                  (rsz (defstobj-fnname field :resize :array renaming))
+                  (acc (defstobj-fnname field :accessor :array renaming))
+                  (len (defstobj-fnname field :length :array renaming))
+                  (field-rec
+                   (defstobj-fnname field :recognizer :hash-table renaming))
+                  (stobj-rec
+                   (defstobj-fnname stobj :recognizer :top renaming))
+                  (init (cadr (assoc-keyword :initially (cdr spec))))
+                  (type (cadr (cadr (assoc-keyword :type (cdr spec)))))
+                  (pred (translate-declaration-to-guard type 'x (w state)))
+                  (stobj-rec-upd-form
+                   `(implies (and (,stobj-rec ,stobj)
+                                  ,pred
+                                  (< (nfix i) (,len ,stobj)))
+                             (,stobj-rec (,upd i x ,stobj)))))
+             (er-let*
+              ((stobj-rec-upd-thms
+                (simplify-thm-fn
+                 (incat field (symbol-name stobj-rec) "-" (symbol-name upd))
+                 stobj-rec-upd-form `(("Goal" :in-theory (theory 'minimal-theory)))
+                 nil state)))
+              (value
+               `((defthmd ,(incat field (symbol-name stobj) "-" 
+                                  (symbol-name field-rec) "-NTH-TYPE")
+                   (implies (and (,field-rec x)
+                                 (< (nfix n) (len x)))
+                            ,(subst '(nth n x) 'x pred))
+                   :rule-classes :type-prescription)
+                 (defthm ,(incat field (symbol-name stobj) "-"
+                                 (symbol-name acc) "-TYPE")
+                   (implies (and (,stobj-rec ,stobj)
+                                 (< (nfix i) (,len ,stobj)))
+                            ,(subst `(,acc i ,stobj) 'x pred))
+                   :hints (("goal" :in-theory
+                            (enable ,(incat field (symbol-name stobj) "-" 
+                                            (symbol-name field-rec)
+                                            "-NTH-TYPE"))))
+                   :rule-classes :type-prescription)
+                 (defthm ,(incat field (symbol-name stobj) "-"
+                                 (symbol-name field-rec) "-UPDATE-NTH")
+                   (implies (and (,field-rec fld)
+                                 (< (nfix n) (len fld))
+                                 ,pred)
+                            (,field-rec (update-nth n x fld))))
+                 ,@stobj-rec-upd-thms
+                 (defthm ,(incat field (symbol-name stobj) "-"
+                                 (symbol-name len) "-TYPE")
+                   (natp (,len ,stobj))
+                   :rule-classes :type-prescription)
+                 (defthm ,(incat field (symbol-name stobj) "-"
+                                 (symbol-name field-rec) "-RESIZE-LIST")
+                   (implies (,field-rec x)
+                            (,field-rec (resize-list x n ,init))))
+                 (defthm ,(incat field (symbol-name stobj) "-"
+                                 (symbol-name rsz) "-" (symbol-name stobj-rec))
+                   (implies (,stobj-rec ,stobj)
+                            (,stobj-rec (,rsz n ,stobj)))))))))
+          (t (let* ((upd (defstobj-fnname field :updater nil renaming))
+                    (acc (defstobj-fnname field :accessor nil renaming))
+                    (type (cadr (assoc-keyword :type (cdr spec))))
+                    (pred (translate-declaration-to-guard type 'x (w state)))
+                    (stobj-rec
+                     (defstobj-fnname stobj :recognizer :top renaming))
+                    (stobj-rec-upd-form
+                     `(implies (and (,stobj-rec ,stobj)
+                                    ,@(if (equal pred ''nil) nil (list pred)))
+                               (,stobj-rec (,upd x ,stobj)))))
+               (er-let*
+                ((stobj-rec-upd-thms
+                  (simplify-thm-fn
+                   (incat field (symbol-name stobj-rec) "-" (symbol-name upd))
+                   stobj-rec-upd-form '(("Goal" :in-theory (theory
+                                                            'minimal-theory)))
+                   nil state)))
+                (if (equal pred ''nil)
+                    (value stobj-rec-upd-thms)
+                  (value
+                   `((defthm ,(incat field (symbol-name stobj) "-" (symbol-name acc) "-TYPE")
+                       (implies (,stobj-rec ,stobj)
+                                ,(subst `(,acc ,stobj) 'x pred))
+                       :rule-classes :type-prescription)
+                     . ,stobj-rec-upd-thms)))))))))
+      (rest (def-stobj-type-theory-fn stobj (cdr specs) renaming state)))
+     (value (append thms rest)))))
+
+
+(defun def-stobj-simple-field-equivs11 (stobj equiv calls)
+  (if (atom calls)
+      nil
+    (cons `(defthm ,(incat equiv (symbol-name equiv) "-"
+                           (symbol-name (caar calls)))
+             (,equiv ,(car calls) ,stobj))
+          (def-stobj-simple-field-equivs11 stobj equiv (cdr calls)))))
+
+(defun def-stobj-simple-field-equivs1 (stobj cspec equiv specs renaming)
+  (if (atom specs)
+      nil
+    (if (equal cspec (car specs))
+        (def-stobj-simple-field-equivs1 stobj cspec equiv (cdr specs) renaming)
+      (let* ((spec (car specs))
+             (calls (mutator-calls spec stobj renaming)))
+        (append (def-stobj-simple-field-equivs11 stobj equiv calls)
+                (def-stobj-simple-field-equivs1 stobj cspec equiv (cdr specs)
+                  renaming))))))
+
+(defun def-stobj-simple-field-equivs (stobj specs all-specs renaming)
+  (if (atom specs)
+      nil
+    (if (or (ht-specp (car specs))
+            (array-specp (car specs)))
+        (def-stobj-simple-field-equivs stobj (cdr specs) all-specs renaming)
+      (let* ((spec (car specs))
+             (field (car spec))
+             (equiv (incat stobj (symbol-name stobj) "-"
+                           (symbol-name field) "-EQ"))
+             (acc (defstobj-fnname field :accessor nil renaming))
+             (upd (defstobj-fnname field :updater nil renaming)))
+        `((defun ,equiv (a b)
+            (declare (xargs :non-executable t))
+            (equal (,acc a) (,acc b)))
+          (defequiv ,equiv)
+          (defcong ,equiv equal (,acc ,stobj) 1)
+          (defthm ,(incat stobj (symbol-name equiv) "-"
+                          (symbol-name upd) "-NORM")
+            (implies (syntaxp (not (equal ,stobj ''t)))
+                     (,equiv (,upd x ,stobj)
+                             (,upd x t))))
+          ,@(def-stobj-simple-field-equivs1 stobj spec equiv all-specs renaming)
+          ,@(def-stobj-simple-field-equivs stobj (cdr specs) all-specs
+              renaming)
+          (in-theory (disable ,equiv)))))))
+             
+             
+
+(defun def-stobj-theory-fn-names1 (specs stobj renaming)
+  (if (atom specs)
+      nil
+    (append
+     (strip-cars (mutator-calls (car specs) stobj renaming))
+     (strip-cars (accessor-calls (car specs) stobj renaming))
+     (def-stobj-theory-fn-names1 (cdr specs) stobj renaming))))
+
+(defun def-stobj-theory-fn-names (specs stobj renaming)
+  (list* (defstobj-fnname stobj :recognizer :top renaming)
+         (def-stobj-theory-fn-names1 specs stobj renaming)))
+
+
+(defun def-stobj-theory-mkevent (stobj state)
+  (declare (xargs :mode :program
+                  :stobjs state))
+  (let* ((rb (getprop stobj 'redundancy-bundle nil 'current-acl2-world
+                      (w state)))
+         (specs (car rb))
+         (renaming (cdr rb))
+         (fn-names (def-stobj-theory-fn-names specs stobj renaming)))
+    (er-let*
+     ((type-thms (def-stobj-type-theory-fn stobj specs renaming state)))
+     (value 
+      `(encapsulate
+        nil
+        ,@(def-stobj-acc-of-upd-thms1 stobj specs specs renaming)
+        ,@type-thms
+        (in-theory (disable . ,fn-names))
+        . ,(def-stobj-simple-field-equivs stobj specs specs renaming))))))
+
+(defmacro def-stobj-theory (stobj)
+  `(make-event
+    (def-stobj-theory-mkevent ',stobj state)))
+
