books/tools/with-arith4-help.lisp
@@ -1,0 +1,62 @@
+
+
+(in-package "ACL2")
+
+(include-book "tools/rulesets" :dir :system)
+
+;; This is included so that this book will be considered dependent on
+;; arith4-theory, so that any books that include this will be considered
+;; dependent on arith4-theory.
+(local (include-book "arith4-theory"))
+
+(defmacro allow-arith4-help ()
+  `(progn
+     (local (include-book
+             "tools/arith4-theory" :dir :system))
+     (defmacro with-arith4-help (&rest stuff)
+       `(encapsulate
+         nil
+         (local (in-theory (e/d* ((:ruleset arith4-enable-ruleset))
+                                 ((:ruleset arith4-disable-ruleset)))))
+;;          (local (table theory-invariant-table nil
+;;                        (table-alist 'post-arith4-theory-invariants world)))
+         . ,stuff))
+
+     (defmacro with-arith4-nonlinear-help (&rest stuff)
+       `(encapsulate
+         nil
+         (local (in-theory (e/d* ((:ruleset arith4-enable-ruleset))
+                                 ((:ruleset arith4-disable-ruleset)))))
+         (local (set-default-hints '((nonlinearp-default-hint
+                                      stable-under-simplificationp
+                                      hist pspv))))
+         (local (table theory-invariant-table nil
+                       (table-alist 'post-arith4-theory-invariants world)
+                       :clear))
+         . ,stuff))
+
+     (defmacro with-arith4-nonlinear++-help (&rest stuff)
+       `(encapsulate
+         nil
+         (local (in-theory (e/d* ((:ruleset arith4-enable-ruleset))
+                                 ((:ruleset arith4-disable-ruleset)))))
+         (local (set-default-hints '((nonlinearp-default-hint
+                                      stable-under-simplificationp
+                                      hist pspv))))
+         (local (table theory-invariant-table nil
+                       (table-alist 'post-arith4-theory-invariants world)
+                       :clear))
+         . ,stuff))))
+
+
+;; Notes:
+
+;; This book allows the arithmetic-4 library to be included locally within a book
+;; while only affecting (i.e. arithmetically helping and slowing down proofs of)
+;; forms that are surrounded by (with-arith4-help  ...).  To allow this:
+
+;; (include-book "tools/with-arith4-help" :dir :system)
+
+;; ;; Locally includes arithmetic-4, reverts to the pre-arithmetic-4 theory,
+;; and defines the with-arith4-help macro.
+;; (allow-arith4-help)
